prove equivalence between big/small semantics

CSL.v
@@ -21,769 +21,513 @@ Require Export Vbase Varith Vlistbase Vlist Basic.
 Set Implicit Arguments.
 Unset Strict Implicit.
 
-Module PHeap.
-  Definition pheap' := Z -> option (Qc * Z).
+Require Import PHeap.
 
-  Definition is_pheap (h : pheap') : Prop :=
-    forall x, match h x with
-      | None => True
-      | Some (p, v) => 0 < p /\ p <= 1
-    end.
-  Record pheap := Pheap { this :> pheap'; is_p : is_pheap this }.
-  Definition pdisj (h1 h2 : pheap') :=
-    forall (x : Z), match h1 x, h2 x with
-      | None, _ | _, None => True
-      | Some (p1, v1), some (p2, v2) =>
-        v1 = v2 /\ 0 < p1 + p2 /\ p1 + p2 <= 1
-    end.
+Definition var := Z.
+Definition stack := var -> Z.
+Definition state := (stack * heap)%type.
 
-  Definition phplus (h1 h2 : pheap') : pheap' :=
-    fun x => match h1 x with
-     | None => h2 x
-     | Some (p1, v1) => 
-       match h2 x with
-         | None => h1 x
-         | Some (p2, v2) => Some (p1 + p2, v1)
-       end
-     end.
+Inductive exp := 
+| Evar (x : var)
+| Enum (n : Z)
+| Eplus (e1: exp) (e2: exp).
 
-  Definition full_p : Qc := 1.
-  Definition emp_h : pheap' := fun (n : Z) => None.
+Inductive bexp :=
+| Beq (e1: exp) (e2: exp)
+| Band (b1: bexp) (b2: bexp)
+| Bnot (b: bexp).
 
-  Definition fpdom (h : pheap') : Prop :=
-    forall (n : Z), match h n with
-      | None => True
-      | Some (p, v) => (p = full_p)%Qc
-    end.
-  
-  Lemma pdisjC : forall h1 h2, pdisj h1 h2 -> pdisj h2 h1.
-  Proof. 
-    unfold pdisj, pheap'; intros h1 h2 hd x.
-    specialize (hd x).
-    destruct (h1 x), (h2 x); try tauto.
-    destruct p as [? ?], p0 as [? ?].
-    assert (q0 + q = q + q0) as heq by ring; rewrite heq.
-    destruct hd as [? [? ?]]; repeat split; auto.
-  Qed.
+Inductive cmd : Set :=
+| Cskip
+| Cassign (x: var) (e: exp)
+| Cread (x: var) (e: exp)
+| Cwrite (e1: exp) (e2: exp)
+| Cseq (c1: cmd) (c2: cmd)
+| Cif (b: bexp) (c1: cmd) (c2: cmd)
+| Cwhile (b: bexp) (c: cmd)
+| Cbarrier (j : nat).
 
-  Lemma pdisj_empty1 : forall (h : pheap), pdisj emp_h h.
-    intros h; unfold emp_h, pdisj; simpl; eauto.
-  Qed.
+Notation "'SKIP'" := Cskip.
+Notation "x '::=' a" := (Cassign x a) (at level 60).
+Notation "x '::=' '[' a ']'" := (Cread x a) (at level 60).
+Notation "'[' a ']' '::=' e" := (Cwrite a e) (at level 60).
+Notation "c1 ;; c2" := (Cseq c1 c2) (at level 80, right associativity).
+Notation "'BARRIER' ( j )" := (Cbarrier j).
 
-  Lemma pdisj_empty2 : forall (h : pheap), pdisj h emp_h.
-     now unfold emp_h, pdisj; intros h x; destruct (this h x) as [[? ?] | ?].
-  Qed.
+Fixpoint wait (c : cmd) : option (nat * cmd) :=
+  match c with
+    | SKIP | _ ::= _ | _ ::= [_] | [_] ::= _ | Cif _ _ _ | Cwhile _ _ => None
+    | BARRIER (j) => Some (j, Cskip)
+    | c1 ;; c2 =>
+      match wait c1 with
+        | Some (j, c1') => Some (j, c1' ;; c2)
+        | None => None
+      end
+  end.
 
-  Definition ph_upd (h : pheap') (x : Z) (v : Z) : pheap' :=
-    fun (x' : Z) => if Z.eq_dec x x' then Some (full_p, v) else h x'.
+Fixpoint edenot e s :=
+  match e with
+    | Evar v => s v
+    | Enum n => n
+    | Eplus e1 e2 => (edenot e1 s + edenot e2 s)%Z
+  end.
 
-  Definition empty_p := 0.
+Fixpoint bdenot b s : bool := 
+  match b with
+    | Beq e1 e2 => if Z.eq_dec (edenot e1 s) (edenot e2 s) then true else false
+    | Band b1 b2 => bdenot b1 s && bdenot b2 s
+    | Bnot b => negb (bdenot b s)
+  end.
 
-  Lemma frac_contra1 : forall p : Qc, (p > empty_p)%Qc -> ~(full_p + p <= full_p)%Qc.
-  Proof.
-    unfold full_p; intros p hp hcontra.
-    apply (Qcle_minus_iff (1 + p) 1) in hcontra.
-    assert (1 + - (1 + p) = -p) as h by ring; rewrite h in hcontra; clear h.
-    apply Qcopp_le_compat in hcontra.
-    assert (- -p = p) as h by ring; rewrite h in hcontra; clear h.
-    assert (- 0 = 0) as h by ring; rewrite h in hcontra; clear h.
-    apply Qclt_not_le in hp; tauto.
-  Qed.
-
-  Lemma frac_contra2 : forall p, p > empty_p -> ~(p + full_p <= 1).
-  Proof.
-    intros ? ?; rewrite Qcplus_comm.
-    auto using frac_contra1.
-  Qed.
-  
-  Lemma pdisj_upd : forall (h h' : pheap) (x w v : Z), this h x = Some (full_p, w) -> 
-    (pdisj (ph_upd h x v) h' <-> pdisj h h').
-  Proof.
-    destruct h as [h iph].
-    destruct h' as [h' iph'].
-    unfold pdisj, ph_upd; ins.
-    split. 
-    - intros hp x0; pose proof (hp x0); pose proof (iph x0); pose proof (iph' x0).
-      destruct (Z.eq_dec x x0), (h x0) as [[? ?] | ], (h' x0) as [[? ?] | ]; eauto.
-      destruct H0 as [? [? ?]],  H2 as [? ?]; exfalso; eapply (@frac_contra1 q0); eauto.
-    - intros hp x0; specialize (hp x0); specialize (iph x0); specialize (iph' x0).
-      destruct (Z.eq_dec x x0); subst;
-      destruct (h x0) as [[? ?] | ], (h' x0) as [[? ?] | ]; simpl; eauto;
-      inversion H; subst.
-      destruct hp as [? [? ?]], iph' as [? ?]; exfalso; eapply (@frac_contra1 q0); eauto.
-  Qed.
-
-  Lemma phplus_comm (h1 h2 : pheap) : pdisj h1 h2 -> phplus h1 h2 = phplus h2 h1.
-  Proof.
-    destruct h1 as [h1 H1], h2 as [h2 H2]; simpl.
-    intros hdisj; unfold is_pheap, pdisj, phplus in *; extensionality x.
-    repeat (match goal with [H : forall _ : Z, _ |- _] => specialize (H x) end).
-    destruct (h1 x) as [[? ?] | ], (h2 x) as [[? ?] | ]; eauto. 
-    destruct hdisj as [? [? ?]].
-    assert (q + q0 = q0 + q) by ring; congruence.
-  Qed.
-
-  Lemma plus_gt_0 : forall p1 p2 : Qc, 0 < p1 -> 0 < p2 -> 0 < p1 + p2.
-  Proof.
-    intros p1 p2 h1 h2.
-    assert (p2 < p1 + p2).
-    { apply Qclt_minus_iff.
-      cutrewrite (p1 + p2 + - p2 = p1); [eauto | ring]. }
-    apply (Qclt_trans _ p2 _); eauto.
-  Qed.
-
-  Lemma gt_0_plus : forall p p1 : Qc, 0 < p1 -> p < p + p1.
-  Proof.
-    intros p p1 h1.
-    apply Qclt_minus_iff.
-    cutrewrite (p + p1 + - p = p1); [eauto | ring].
-  Qed.
-
-  Lemma le1_weak : forall p p1 : Qc, 0 < p1 -> p + p1 <= 1 -> p <= 1.
-  Proof.
-    intros p p1 h1 hp.
-    apply Qclt_le_weak.
-    apply (Qclt_le_trans _ (p + p1) _); [apply gt_0_plus; eauto | eauto].
-  Qed.
-
-  Lemma pdisj_padd (h1 h2 h3 : pheap) :
-    pdisj h2 h3 -> pdisj h1 (phplus h2 h3) -> (pdisj h1 h2) /\ (pdisj h1 h3).
-  Proof.
-    destruct h1 as [h1 H1], h2 as [h2 H2], h3 as [h3 H3]; simpl.
-    unfold is_pheap, pdisj, phplus in *;
-    intros disj23 disj123; split; intros x; 
-    repeat (match goal with [H : forall _ : Z, _ |- _] => specialize (H x) end);
-    destruct (h1 x) as [[? ?] |], (h2 x) as [[? ?] |], (h3 x) as [[? ?] |];
-    destruct disj23 as [? [? ?]], disj123 as [? [? ?]], H1 as [? ?], H2 as [? ?], H3 as [? ?];
-    repeat split; eauto using Qcplus_comm.
-
-    - apply plus_gt_0; eauto.
-    - cutrewrite (q + (q0 + q1) = (q + q0) + q1) in H7; [apply (@le1_weak _ q1); eauto | ring ].
-    - congruence.
-    - apply plus_gt_0; eauto.
-    - cutrewrite (q + (q0 + q1) = (q + q1) + q0) in H7; [apply (@le1_weak _ q0); eauto | ring ].
-  Qed.
-
-  Lemma pdisjE1 (h1 h2 h3 : pheap) : pdisj h1 (phplus h2 h3) -> pdisj h2 h3 -> pdisj h1 h2.
-  Proof.
-    destruct h1 as [h1 ph1], h2 as [h2 ph2], h3 as [h3 ph3]; simpl in *.
-    unfold is_pheap, pdisj, phplus in *;
-    intros h123 h23 x;
-    repeat (match goal with [H : forall _ : Z, _ |- _] => specialize (H x) end).
-    destruct (h1 x) as [[? ?] |], (h2 x) as [[? ?] |], (h3 x) as [[? ?] |],
-             ph1 as [? ?], ph2 as [? ?], ph3 as [? ?], h123 as [? [? ?]], h23 as [? [? ?]]; eauto.
-    repeat split; eauto using plus_gt_0.
-    cutrewrite (q + (q0 + q1) = (q + q0) + q1) in H7; [apply (@le1_weak _ q1); eauto | ring ].
-  Qed.
-
-  Lemma pdisjE2 (h1 h2 h3 : pheap) :
-    pdisj h1 (phplus h2 h3) -> pdisj h2 h3 -> pdisj h1 h3.
-  Proof.
-    destruct h1 as [h1 ph1], h2 as [h2 ph2], h3 as [h3 ph3]; simpl in *.
-    unfold is_pheap, pdisj, phplus in *;
-    intros h123 h23 x;
-    repeat (match goal with [H : forall _ : Z, _ |- _] => specialize (H x) end).
-    destruct (h1 x) as [[? ?] |], (h2 x) as [[? ?] |], (h3 x) as [[? ?] |],
-             ph1 as [? ?], ph2 as [? ?], ph3 as [? ?], h123 as [? [? ?]], h23 as [? [? ?]]; eauto.
-    repeat split; eauto using plus_gt_0.
-    - congruence.
-    - cutrewrite (q + (q0 + q1) = (q + q1) + q0) in H7; [apply (@le1_weak _ q0); eauto | ring ].
-  Qed.
-
-  Lemma pdisj_padd_comm (h1 h2 h3 : pheap) : pdisj h2 (phplus h1 h3) -> pdisj h1 h3 -> 
-                                             pdisj h1 (phplus h2 h3).
-  Proof.
-    destruct h1 as [h1 ph1], h2 as [h2 ph2], h3 as [h3 ph3]; simpl in *.
-    unfold is_pheap, pdisj, phplus in *;
-    intros h123 h23 x;
-    repeat (match goal with [H : forall _ : Z, _ |- _] => specialize (H x) end).
-    destruct (h1 x) as [[? ?] |], (h2 x) as [[? ?] |], (h3 x) as [[? ?] |],
-             ph1 as [? ?], ph2 as [? ?], ph3 as [? ?], h123 as [? [? ?]], h23 as [? [? ?]]; eauto.
-    - cutrewrite (q + (q0 + q1) = q0 + (q + q1)); [ | ring].
-      repeat split; eauto.
-    - cutrewrite (q + q0 = q0 + q); [ | ring];
-      repeat split; eauto.
-  Qed.
-
-  Lemma pdisj_padd_expand 
-        (h1 h2 h3 : pheap) : pdisj h1 h2 -> 
-                             (pdisj (phplus h1 h2) h3 <-> (pdisj h1 (phplus h2 h3) /\ pdisj h2 h3)).
-  Proof.
-    destruct h1 as [h1 ph1], h2 as [h2 ph2], h3 as [h3 ph3]; simpl in *.
-    unfold is_pheap, pdisj, phplus in *;
-    intros h12; split; [intros H; split; intros x | intros [H1 H2] x];
-    repeat (match goal with [H : forall _ : Z, _ |- _] => specialize (H x) end);
-    destruct (h1 x) as [[? ?] |], (h2 x) as [[? ?] |], (h3 x) as [[? ?] |],
-             ph1 as [? ?], ph2 as [? ?], ph3 as [? ?], h12 as [? [? ?]];
-    des; eauto;
-    repeat split; try congruence; eauto; 
-    try rewrite (Qcplus_assoc _ _ _); try rewrite (Qcplus_comm _ _); 
-    eauto using plus_gt_0.
-    - cutrewrite (q1 + (q + q0) = q + q0 + q1); [eauto | ring].
-    - cutrewrite (q + q0 + q1 = (q1 + q0) + q) in H10; [apply (@le1_weak _ q); eauto | ring].
-    - cutrewrite (q1 + (q + q0) = q + (q0 + q1)); [eauto | ring].
-  Qed.
-
-  Lemma padd_assoc
-        (h1 h2 h3 : pheap)  :
-    pdisj h1 (phplus h2 h3) -> pdisj h2 h3 -> phplus (phplus h1 h2) h3 = phplus h1 (phplus h2 h3).
-  Proof.
-    destruct h1 as [h1 ph1], h2 as [h2 ph2], h3 as [h3 ph3]; simpl in *.
-    unfold is_pheap, pdisj, phplus in *;
-    intros h123 h23; extensionality x;
-    repeat (match goal with [H : forall _ : Z, _ |- _] => specialize (H x) end);
-    destruct (h1 x) as [[? ?] |], (h2 x) as [[? ?] |], (h3 x) as [[? ?] |];
-    des; eauto.
-    cutrewrite (q + q0 + q1 = q + (q0 + q1)); [eauto | ring].
-  Qed.
-
-  Lemma padd_left_comm 
-        (h1 h2 h3 : pheap) :
-    pdisj h1 (phplus h2 h3) -> pdisj h2 h3 -> phplus h1 (phplus h2 h3) = phplus h2 (phplus h1 h3).
-  Proof.
-    destruct h1 as [h1 ph1], h2 as [h2 ph2], h3 as [h3 ph3]; simpl in *.
-    unfold is_pheap, pdisj, phplus in *;
-    intros h123 h23; extensionality x;
-    repeat (match goal with [H : forall _ : Z, _ |- _] => specialize (H x) end);
-    destruct (h1 x) as [[? ?] |], (h2 x) as [[? ?] |], (h3 x) as [[? ?] |];
-    des; eauto.
-    - cutrewrite (q + (q0 + q1) = q0 + (q + q1)); [congruence | ring].
-    - cutrewrite (q + q0 = q0 + q); [congruence | ring].
-  Qed.
-  
-  Lemma padd_cancel
-        (h1 h2 h3 : pheap) :
-    phplus h1 h2 = phplus h1 h3 -> pdisj h1 h2 -> pdisj h1 h3 -> h2 = h3.
-  Proof.
-    destruct h1 as [h1 ph1], h2 as [h2 ph2], h3 as [h3 ph3]; simpl in *.
-    intros heq h12 h13.
-    assert (h2 = h3).
-    unfold is_pheap, pdisj, phplus in *;
-    extensionality x; pose proof  (equal_f heq x) as heq'; simpl in *; clear heq;
-    repeat (match goal with [H : forall _ : Z, _ |- _] => specialize (H x) end);
-    destruct (h1 x) as [[? ?] |], (h2 x) as [[? ?] |], (h3 x) as [[? ?] |];
-    des; eauto; try congruence.
-    - remember (q + q0) as q0'; remember (q + q1) as q1'.
-      inversion heq'. subst.
-      assert (q + q0 - q = q + q1 - q) by (rewrite H0; eauto).
-      cutrewrite (q + q0 - q = q0) in H; [| ring].
-      cutrewrite (q + q1 - q = q1) in H; [| ring].
-      congruence.
-    - remember (q + q0) as q'.
-      inversion heq'; subst.
-      assert (q + q0 - q = q - q) by (rewrite H0; eauto).
-      cutrewrite (q + q0 - q = q0) in H; [| ring].
-      cutrewrite (q - q = 0) in H; [| ring].
-      rewrite H in ph2.
-      inversion ph2.
-    - inversion heq'.
-      assert (q - q = (q + q0) - q) by (rewrite H0 at 1; eauto).
-      cutrewrite (q - q = 0) in H; [| ring].
-      cutrewrite (q + q0 - q = q0) in H; [| ring].
-      rewrite <- H in ph3; inversion ph3.
-    - subst; cutrewrite (ph2 = ph3); [eauto | apply proof_irrelevance ].
-  Qed.
-
-  Corollary padd_cancel2 (h1 h2 h3 : pheap) :
-    phplus h2 h1 = phplus h3 h1 -> pdisj h2 h1 -> pdisj h3 h1 -> h2 = h3.
-  Proof.
-    Hint Resolve pdisjC.
-    intros.
-    rewrite (@phplus_comm h2 h1), (@phplus_comm h3 h1) in H; eauto.
-    eapply padd_cancel; eauto.
-  Qed.
-
-  Definition ptoheap (ph : pheap') (h : heap) : Prop :=
-    forall (x : Z), match ph x with
-      | None => h x = None
-      | Some (p, v) => p = full_p /\ h x = Some v
-    end.
-
-  Lemma ptoD (ph1 ph2 : pheap') (h : heap):
-    ptoheap ph1 h -> ptoheap ph2 h -> ph1 = ph2.
-  Proof.
-(*    destruct ph1 as [h1 ph1], ph2 as [h2 ph2]; simpl in *.*)
-    intros pto1 pto2.
-    unfold is_pheap, pdisj, phplus, ptoheap in *; extensionality x; simpl in *;
-    repeat (match goal with [H : forall _ : Z, _ |- _] => specialize (H x) end);
-    destruct (ph1 x) as [[? ?] |], (ph2 x) as [[? ?] |];
-    des; eauto; try congruence.
-  Qed.
-End PHeap.
-
-Module Language.
-  Import PHeap.
-  
-  Definition var := Z.
-  Definition stack := var -> Z.
-  Definition state := (stack * heap)%type.
-
-  Inductive exp := 
-  | Evar (x : var)
-  | Enum (n : Z)
-  | Eplus (e1: exp) (e2: exp).
-
-  Inductive bexp :=
-  | Beq (e1: exp) (e2: exp)
-  | Band (b1: bexp) (b2: bexp)
-  | Bnot (b: bexp).
-
-  Inductive cmd : Set :=
-  | Cskip
-  | Cassign (x: var) (e: exp)
-  | Cread (x: var) (e: exp)
-  | Cwrite (e1: exp) (e2: exp)
-  | Cseq (c1: cmd) (c2: cmd)
-  | Cif (b: bexp) (c1: cmd) (c2: cmd)
-  | Cwhile (b: bexp) (c: cmd)
-  | Cbarrier (j : nat).
-
-  Notation "'SKIP'" := Cskip.
-  Notation "x '::=' a" := (Cassign x a) (at level 60).
-  Notation "x '::=' '[' a ']'" := (Cread x a) (at level 60).
-  Notation "'[' a ']' '::=' e" := (Cwrite a e) (at level 60).
-  Notation "c1 ;; c2" := (Cseq c1 c2) (at level 80, right associativity).
-  Notation "'BARRIER' ( j )" := (Cbarrier j).
-
-  Fixpoint wait (c : cmd) : option (nat * cmd) :=
-    match c with
-      | SKIP | _ ::= _ | _ ::= [_] | [_] ::= _ | Cif _ _ _ | Cwhile _ _ => None
-      | BARRIER (j) => Some (j, Cskip)
-      | c1 ;; c2 =>
-        match wait c1 with
-          | Some (j, c1') => Some (j, c1' ;; c2)
-          | None => None
-        end
-    end.
-
-  Fixpoint edenot e s :=
-    match e with
-      | Evar v => s v
-      | Enum n => n
-      | Eplus e1 e2 => (edenot e1 s + edenot e2 s)%Z
-    end.
-  
-  Fixpoint bdenot b s : bool := 
-    match b with
-      | Beq e1 e2 => if Z.eq_dec (edenot e1 s) (edenot e2 s) then true else false
-      | Band b1 b2 => bdenot b1 s && bdenot b2 s
-      | Bnot b => negb (bdenot b s)
-    end.
-  
-  Reserved Notation "c '/' st  '==>s'  c' '/' st' " (at level 40, st at level 39, c' at level 39).
-  Inductive red: cmd -> state -> cmd  -> state -> Prop := 
-  | red_Seq1: forall (c : cmd) (ss : state), (SKIP ;; c) / ss ==>s c / ss
-  | red_Seq2: forall (c1 : cmd) (ss : state) (c1' : cmd) (ss' : state) (c2 : cmd)
-                     (R: c1 / ss ==>s c1' / ss'), 
-                   (c1 ;; c2) / ss ==>s (c1' ;; c2) / ss'
-  | red_If1: forall (b : bexp) (c1 c2 : cmd) (ss : state) 
-                    (B: bdenot b (fst ss) = true), 
-                    (Cif b c1 c2) / ss ==>s c1 / ss
-  | red_If2: forall (b : bexp) (c1 c2 : cmd) (ss : state)
-                    (B: bdenot b (fst ss) = false),
-                    (Cif b c1 c2) / ss ==>s c2 / ss
-  | red_Loop: forall (b : bexp) (c : cmd) (ss : state), 
-                    (Cwhile b c) / ss ==>s (Cif b (Cseq c (Cwhile b c)) Cskip) / ss
-  | red_Assign: forall (x : var) (e : exp) ss ss' s h
-                       (EQ1: ss = (s, h))
-                       (EQ2: ss' = (upd s x (edenot e s), h)),
-                       (x ::= e) / ss ==>s Cskip / ss'
-  | red_Read: forall x e ss ss' s h v
+Reserved Notation "c '/' st  '==>s'  c' '/' st' " (at level 40, st at level 39, c' at level 39).
+Inductive red: cmd -> state -> cmd  -> state -> Prop := 
+| red_Seq1: forall (c : cmd) (ss : state), (SKIP ;; c) / ss ==>s c / ss
+| red_Seq2: forall (c1 : cmd) (ss : state) (c1' : cmd) (ss' : state) (c2 : cmd)
+                   (R: c1 / ss ==>s c1' / ss'), 
+              (c1 ;; c2) / ss ==>s (c1' ;; c2) / ss'
+| red_If1: forall (b : bexp) (c1 c2 : cmd) (ss : state) 
+                  (B: bdenot b (fst ss) = true), 
+             (Cif b c1 c2) / ss ==>s c1 / ss
+| red_If2: forall (b : bexp) (c1 c2 : cmd) (ss : state)
+                  (B: bdenot b (fst ss) = false),
+             (Cif b c1 c2) / ss ==>s c2 / ss
+| red_Loop: forall (b : bexp) (c : cmd) (ss : state), 
+              (Cwhile b c) / ss ==>s (Cif b (Cseq c (Cwhile b c)) Cskip) / ss
+| red_Assign: forall (x : var) (e : exp) ss ss' s h
                      (EQ1: ss = (s, h))
-                     (RD: h (edenot e s) = Some v)
-                     (EQ2: ss' = (upd s x v, h)),
-                     (x ::= [e]) / ss ==>s Cskip / ss'
-  | red_Write: forall e1 e2 ss ss' s h
-                      (EQ1: ss = (s, h))
-                      (EQ2: ss' = (s, upd h (edenot e1 s) (Some (edenot e2 s)))),
-                      (Cwrite e1 e2) / ss ==>s Cskip / ss'
-   where  "c '/' st  '==>s'  c' '/' st' " := (red c st c' st').
+                     (EQ2: ss' = (upd s x (edenot e s), h)),
+                (x ::= e) / ss ==>s Cskip / ss'
+| red_Read: forall x e ss ss' s h v
+                   (EQ1: ss = (s, h))
+                   (RD: h (edenot e s) = Some v)
+                   (EQ2: ss' = (upd s x v, h)),
+              (x ::= [e]) / ss ==>s Cskip / ss'
+| red_Write: forall e1 e2 ss ss' s h
+                    (EQ1: ss = (s, h))
+                    (EQ2: ss' = (s, upd h (edenot e1 s) (Some (edenot e2 s)))),
+               (Cwrite e1 e2) / ss ==>s Cskip / ss'
+                              where  "c '/' st  '==>s'  c' '/' st' " := (red c st c' st').
 
-  Definition red_tup (st1 st2 : (cmd * state)) : Prop := red (fst st1) (snd st1) (fst st2) (snd st2).
-  Definition multi_red_tup : (cmd * state) -> (cmd * state) -> Prop := clos_refl_trans_1n _ red_tup.
-  Definition multi_red (c1 : cmd) (st1 : state) (c2 : cmd) (st2 : state) := 
-    multi_red_tup (c1, st1) (c2, st2).
+Definition red_tup (st1 st2 : (cmd * state)) : Prop := red (fst st1) (snd st1) (fst st2) (snd st2).
+Definition multi_red_tup : (cmd * state) -> (cmd * state) -> Prop := clos_refl_trans_1n _ red_tup.
+Definition multi_red (c1 : cmd) (st1 : state) (c2 : cmd) (st2 : state) := 
+  multi_red_tup (c1, st1) (c2, st2).
+
+Notation "c '/' st  '==>s*'  c' '/' st' " := (multi_red c st c' st') (at level 40, st at level 39, c' at level 39).
+
+Lemma red_det (c c1 c2 : cmd) (st st1 st2 : state) :
+  c / st ==>s c1 / st1 ->
+  c / st ==>s c2 / st2 ->
+  c1 = c2 /\ st1 = st2.
+Proof.
+  intros red1 red2.
+  induction [c2 st2 red2]red1; intros c2' st2 red2; try (inversion red2; subst; split; congruence).
+  - inversion red2; subst; eauto.
+    inversion R.
+  - inversion red2; subst.
+    + inversion red1.
+    + apply IHred1 in R; destruct R; subst; split; congruence.
+Qed.
+
+Fixpoint accesses (c : cmd) (s : stack) := 
+  match c with
+    | Cskip => None
+    | x ::= e => None
+    | x ::= [e] => Some (edenot e s)
+    | [e] ::= e' => Some (edenot e s)
+    | c1 ;; c2 => accesses c1 s
+    | (Cif b c1 c2) => None
+    | (Cwhile b c) => None
+    | (Cbarrier _) => None
+  end.
+
+Fixpoint writes (c : cmd) (s : stack) :=
+  match c with
+    | Cskip => None
+    | (x ::= e) => None
+    | (x ::= [e]) => None
+    | ([e] ::= e') => Some (edenot e s)
+    | (c1 ;; c2) => writes c1 s
+    | (Cif b c1 c2) => None
+    | (Cwhile b c) => None
+    | Cbarrier j => None
+  end.
+
+Inductive aborts : cmd -> state -> Prop := 
+| aborts_Seq : forall (c1 c2 : cmd) (ss : state) (A: aborts c1 ss), aborts (Cseq c1 c2) ss
+| aborts_Read: forall x e ss
+                      (NIN: snd ss (edenot e (fst ss)) = None),
+                 aborts (Cread x e) ss
+| aborts_Write: forall e1 e2 ss
+                       (NIN: snd ss (edenot e1 (fst ss)) = None),
+                  aborts (Cwrite e1 e2) ss.
+
+Fixpoint barriers c :=
+  match c with
+    | Cskip => nil
+    | (Cassign x e) => nil
+    | (Cread x e) => nil
+    | (Cwrite e e') => nil
+    | (Cseq c1 c2) => barriers c1 ++ barriers c2
+    | (Cif b c1 c2) => barriers c1 ++ barriers c2
+    | (Cwhile b c) => barriers c
+    | Cbarrier j => j :: nil
+  end.
+
+Definition wf_cmd c := disjoint_list (barriers c).
+
+Module PLang.
+  Definition pstate := (stack * pheap)%type.
   
-  Notation "c '/' st  '==>s*'  c' '/' st' " := (multi_red c st c' st') (at level 40, st at level 39, c' at level 39).
+  Definition access_ok (c : cmd) (s : stack) (h : pheap) :=
+    match accesses c s with
+      | None => True
+      | Some v => exists x, this h v = Some x
+    end.
 
-  Lemma red_det (c c1 c2 : cmd) (st st1 st2 : state) :
-    c / st ==>s c1 / st1 ->
-    c / st ==>s c2 / st2 ->
+  Definition write_ok (c : cmd) (s : stack) (h : pheap) :=
+    match writes c s with
+      | None => True
+      | Some v => exists x, this h v = Some (full_p, x)
+    end.
+
+  Inductive red_p: cmd -> pstate -> cmd -> pstate -> Prop :=
+    redp_ster : forall (c1 c2 : cmd) (st1 st2 : state) (pst1 pst2 : pstate) (s1 s2 : stack)
+                       (ph1 ph2 phF : pheap) (h1 h2 : heap),
+                  st1 = (s1, h1) -> st2 = (s2, h2) ->
+                  pst1 = (s1, ph1) -> pst2 = (s2, ph2) ->
+                  access_ok c1 s1 ph1 ->
+                  write_ok c1 s1 ph1 ->
+                  pdisj ph1 phF -> ptoheap (phplus ph1 phF) h1 ->
+                  c1 / st1 ==>s c2 / st2 ->
+                  pdisj ph2 phF -> ptoheap (phplus ph2 phF) h2 ->
+                  red_p c1 pst1 c2 pst2.
+  Notation "c '/' st  '==>p'  c' '/' st' " := 
+    (red_p c st c' st') (at level 40, st at level 39, c' at level 39).
+
+  Definition red_p_tup (st1 st2 : (cmd * pstate)) : Prop := 
+    red_p (fst st1) (snd st1) (fst st2) (snd st2).
+  Definition multi_red_p_tup : (cmd * pstate) -> (cmd * pstate) -> Prop := 
+    clos_refl_trans_1n _ red_p_tup.
+  Definition multi_red_p (c1 : cmd) (st1 : pstate) (c2 : cmd) (st2 : pstate) := 
+    multi_red_p_tup (c1, st1) (c2, st2).
+  
+  Notation "c '/' st  '==>p*'  c' '/' st' " := (multi_red_p c st c' st') 
+    (at level 40, st at level 39, c' at level 39).
+
+  Hint Resolve pdisjC.
+  Lemma Q1 (q1 q2 q : Qc) : q1 + q2 = q -> q1 = q - q2.
+  Proof. intros H; rewrite <-H; ring. Qed.
+  Hint Rewrite Q1.
+
+  Lemma Q2 (q1 q2 q : Qc) : q1 + q2 = q -> q2 = q - q1.
+  Proof. intros H; rewrite <-H; ring. Qed.
+  Hint Rewrite Q2.
+
+  Lemma phplus_cancel_toheap (ph1 ph2 phF : pheap) (h : heap):
+    pdisj ph1 phF -> pdisj ph2 phF ->
+    ptoheap (phplus ph1 phF) h -> ptoheap (phplus ph2 phF) h -> ph1 = ph2.
+  Proof.
+    intros dis1 id2 to1 to2.
+    pose proof (ptoD to1 to2).
+    eapply padd_cancel2; eauto.
+  Qed.
+
+  Lemma padd_upd_cancel (ph1 ph2 phF : pheap) (h : heap) (x v v': Z) :
+    pdisj ph1 phF -> pdisj ph2 phF -> ptoheap (phplus ph1 phF) h ->
+    this ph1 x = Some (full_p, v') -> ptoheap (phplus ph2 phF) (upd h x (Some v)) -> 
+    this ph2 = ph_upd ph1 x v.
+  Proof.
+    intros pd1 pd2 toh1 have1 toh2; extensionality y; unfold ph_upd.
+    destruct ph1 as [ph1 h1], ph2 as [ph2 h2], phF as [phF hF]; simpl in *.
+    destruct (Z.eq_dec x y).
+    - rewrite <-e; clear e y.
+      unfold is_pheap, pdisj, ptoheap, upd, phplus in *;
+        repeat (match goal with [H : forall _ : Z, _ |- _] => specialize (H x) end).
+      destruct (Z.eq_dec x x); try tauto.
+      rewrite have1 in *.
+      destruct (phF x) as [[pF vF]|]; des.
+      + apply Qcle_minus_iff in pd3.
+        cutrewrite (1 + -(full_p + pF) = -pF) in pd3; [|unfold full_p; field].
+        apply Qcopp_le_compat in pd3; ring_simplify in pd3.
+        apply Qcle_not_lt in pd3; tauto.
+      + destruct (ph2 x) as [[p2 v2]|]; try congruence.
+        des; congruence.
+    - unfold is_pheap, pdisj, ptoheap, upd, phplus in *;
+      repeat (match goal with [H : forall _ : Z, _ |- _] => specialize (H y) end).
+      destruct (Z.eq_dec y x); [symmetry in e; tauto |].
+      destruct (ph1 y) as [[? ?]|], (phF y) as [[? ?]|], (ph2 y) as [[? ?]|]; des; 
+      try congruence.
+      apply Q1 in toh1; apply Q1 in toh2.
+      destruct (h y) as [? | ]; inversion toh0; inversion toh3; congruence.
+      rewrite toh2 in toh1.
+      assert (q + full_p - full_p = full_p - full_p) by (rewrite toh1; ring).
+      ring_simplify in H; rewrite H in h1; inversion h1.
+      rewrite toh1 in toh2.
+      assert (q0 + full_p - full_p = full_p - full_p) by (rewrite toh2; ring).
+      ring_simplify in H; rewrite H in h2; inversion h2.
+  Qed.
+
+  Lemma red_p_det (c c1 c2 : cmd) (st st1 st2 : pstate) :
+    c / st ==>p c1 / st1 ->
+    c / st ==>p c2 / st2 ->
     c1 = c2 /\ st1 = st2.
   Proof.
     intros red1 red2.
-    induction [c2 st2 red2]red1; intros c2' st2 red2; try (inversion red2; subst; split; congruence).
-    - inversion red2; subst; eauto.
-      inversion R.
+    destruct red1 as
+        [c1 c1' st1 st1' pst1 pst1' s1 s1' ph1 ph1' phF1 h1 h1' eq1 eq1' 
+            peq1 peq1' aok1 wok1 dis1 to1 red1 dis1' to1'].
+    destruct red2 as
+        [c2 c2' st2 st2' pst2 pst2' s2 s2' ph2 ph2' phF2 h2 h2' eq2 eq2' 
+            peq2 peq2' aok2 wok2 dis2 to2 red2 dis2' to2'].
+    induction [c2' red2]red1; intros c2' red2; 
+    try (inversion red2; subst; 
+         repeat (match goal with [H : (_, _) = (_, _) |- _ ] => inversion H; subst; clear H end);
+         simpl in *; try congruence;
+         assert (ph1' = ph2) by (eapply phplus_cancel_toheap; eauto);
+         assert (ph2' = ph2) by (eapply phplus_cancel_toheap; eauto);
+         split; congruence).
     - inversion red2; subst.
-      + inversion red1.
-      + apply IHred1 in R; destruct R; subst; split; congruence.
-  Qed.
-
-  Fixpoint accesses (c : cmd) (s : stack) := 
-    match c with
-      | Cskip => None
-      | x ::= e => None
-      | x ::= [e] => Some (edenot e s)
-      | [e] ::= e' => Some (edenot e s)
-      | c1 ;; c2 => accesses c1 s
-      | (Cif b c1 c2) => None
-      | (Cwhile b c) => None
-      | (Cbarrier _) => None
-    end.
-
-  Fixpoint writes (c : cmd) (s : stack) :=
-    match c with
-      | Cskip => None
-      | (x ::= e) => None
-      | (x ::= [e]) => None
-      | ([e] ::= e') => Some (edenot e s)
-      | (c1 ;; c2) => writes c1 s
-      | (Cif b c1 c2) => None
-      | (Cwhile b c) => None
-      | Cbarrier j => None
-    end.
-  
-  Inductive aborts : cmd -> state -> Prop := 
-  | aborts_Seq : forall (c1 c2 : cmd) (ss : state) (A: aborts c1 ss), aborts (Cseq c1 c2) ss
-  | aborts_Read: forall x e ss
-                        (NIN: snd ss (edenot e (fst ss)) = None),
-                   aborts (Cread x e) ss
-  | aborts_Write: forall e1 e2 ss
-                         (NIN: snd ss (edenot e1 (fst ss)) = None),
-                    aborts (Cwrite e1 e2) ss.
-
-  Fixpoint barriers c :=
-    match c with
-      | Cskip => nil
-      | (Cassign x e) => nil
-      | (Cread x e) => nil
-      | (Cwrite e e') => nil
-      | (Cseq c1 c2) => barriers c1 ++ barriers c2
-      | (Cif b c1 c2) => barriers c1 ++ barriers c2
-      | (Cwhile b c) => barriers c
-      | Cbarrier j => j :: nil
-    end.
-
-  Definition wf_cmd c := disjoint_list (barriers c).
-
-  Module BigStep.
-    Reserved Notation " c '/' s '||' c' '/' s'" (at level 40, s at level 39, c' at level 39).
-    Inductive eval : cmd -> state -> option (nat * cmd) -> state -> Prop :=
-    | eval_Skip : forall (st : state), SKIP / st || None / st
-    | eval_Seq1 : forall (c1 c2 c1': cmd) (st st' : state) (j : nat),
-                    c1 / st || (Some (j, c1')) / st' ->
-                    (c1 ;; c2) / st || Some (j, c1' ;; c2) / st'
-    | eval_Seq2 : forall (c1 c2 : cmd) (c2' : option (nat * cmd)) (st st' st'' : state), 
-                    c1 / st || None / st' -> c2 / st' || c2' / st'' -> (c1 ;; c2) / st || c2' / st''
-    | eval_If1 : forall (b : bexp) (c1 c2 : cmd) (c1' : option (nat * cmd)) (st st' : state),
-                  bdenot b (fst st) = true -> c1 / st || c1' / st' ->
-                  (Cif b c1 c2) / st || c1' / st'
-    | eval_If2 : forall (b : bexp) (c1 c2 : cmd) (c2' : option (nat * cmd)) (st st' : state),
-                   bdenot b (fst st) = false -> c2 / st || c2' / st' ->
-                   (Cif b c1 c2) / st || c2' / st'
-    | eval_Loop : forall (b : bexp) (c : cmd) (c' : option (nat * cmd)) (st st' : state),
-                     (Cif b (c ;; (Cwhile b c)) Cskip) / st || c'/ st' ->
-                     (Cwhile b c) / st || c' / st'
-    | eval_Assign : forall (x : var) (e : exp) (st st' : state) s h,
-                      (st = (s, h)) -> (st' = (upd s x (edenot e s), h)) ->
-                      (x ::= e) / st || None / st'
-    | eval_Read : forall (x : var) (e : exp) (v : Z) (st st' : state) (s : stack) (h : heap),
-                    (st = (s, h)) -> (h (edenot e s) = Some v) ->
-                    (st' = (upd s x v, h)) ->
-                    (x ::= [e]) / st || None / st'
-    | eval_Write : forall e1 e2 ss ss' s h,
-                     (ss = (s, h)) ->
-                     (ss' = (s, upd h (edenot e1 s) (Some (edenot e2 s)))) ->
-                     (Cwrite e1 e2) / ss || None / ss'
-    | eval_Barrier : forall ss j,
-                       (Cbarrier j) / ss || Some (j, Cskip) / ss
-      where " c '/' s '||' c' '/' s'" := (eval c s c' s').
-    
-    Lemma red1_eval (c1 c2 : cmd) (st1 st2 : state) (st : state) : 
-      c1 / st1 ==>s c2 / st2 -> c2 / st2 || None / st -> c1 / st1 || None / st.
-    Proof.
-      move=> H IH.
-      induction [st IH]H; ins; try do 10 (econstructor; eauto).
-      - inversion IH; subst.
-        econstructor; eauto.
-      - apply eval_If2; eauto.
-      - eapply eval_Assign; eauto.
-        inversion IH; subst; eauto.
-      - eapply eval_Read; eauto.
-        inversion IH; subst; eauto.
-      - eapply eval_Write; eauto.
-        inversion IH; subst; eauto.
-    Qed.
-
-    Corollary red1_eval' (c1 c2 : cmd) (st1 st2 st3 : state) : 
-      c1 / st1 ==>s c2 / st2 -> c2 / st2 || None / st3 -> c1 / st1 || None / st3.
-    Proof.
-      move=> H H'.
-      remember (c1, st1) as s1.
-      assert (c1 = fst s1) as h by (rewrite Heqs1; tauto); rewrite h in *; clear h.
-      assert (st1 = snd s1) as h by (rewrite Heqs1; tauto); rewrite h in *; clear h.
-      remember (c2, st2) as s2.
-      assert (c2 = fst s2) as h by (rewrite Heqs2; tauto); rewrite h in *; clear h.
-      assert (st2 = snd s2) as h by (rewrite Heqs2; tauto); rewrite h in *; clear h.
-      eapply red1_eval; eauto.
-    Qed.
-
-    Lemma eval__mred1 (c : cmd) (st st' : state) : 
-      c / st ==>s* Cskip / st' -> c / st || None / st'.
-      intros H. unfold multi_red in H.
-      remember (c, st) as s.
-      remember (SKIP, st') as s'.
-      assert (c = fst s) as h by (rewrite Heqs; tauto); rewrite h; clear h.
-      assert (st = snd s) as h by (rewrite Heqs; tauto); rewrite h; clear h.
-      assert (st' = snd s') as h by (rewrite Heqs'; tauto); rewrite h; clear h.
-      clear Heqs.
-       induction [Heqs'] H.
-      - move=>->; simpl; apply eval_Skip.
-      - move/IHclos_refl_trans_1n=>IH; clear IHclos_refl_trans_1n.
-        clear H0.
-        eapply red1_eval; eauto.
-    Qed.
-
-    Lemma eval_mred2 (c c' c'': cmd) (st st' : state) (j : nat) : 
-      c / st ==>s* c' / st' -> wait c' = Some (j, c'') ->
-      c / st || Some (j, c'') / st'.
-    Proof.
-      intros hs hwait.
-      unfold multi_red in hs.
-      remember (c, st) as s.
-      remember (c', st') as s'.
-      assert (c = fst s) as h by (rewrite Heqs; tauto); rewrite h; clear h.
-      assert (st = snd s) as h by (rewrite Heqs; tauto); rewrite h; clear h.
-      assert (st' = snd s') as h by (rewrite Heqs'; tauto); rewrite h; clear h.
-      clear Heqs.
-      induction [Heqs'] hs.
-      - intros ->.
-        induction [c'' j hwait]c'; move=> c'' j' hwait; inversion hwait.
-        + destruct (wait c'1); eauto.
-          * destruct p as (j'', c'); simpl in *.
-            apply eval_Seq1.
-            now apply IHc'1.
-          * inversion H0.
-        + apply eval_Barrier.
-      - move=>->; simpl in *.
-        assert ((c', st') = (c', st')) as IH by eauto; apply IHhs in IH; clear IHhs; simpl in *.
-        clear hs hwait c' c st.
-        unfold red_tup in H;
-        induction [c'' IH]H; ins; try do 5 (econstructor; eauto).
-        + inversion IH; subst.
-          * apply eval_Seq1. 
-            apply IHred; eauto.
-          * eapply eval_Seq2; eauto.
-            eapply red1_eval'; eauto.
-        + apply eval_If2; eauto.
-        + inversion IH.
-        + inversion IH.
-        + inversion IH.
-    Qed.
-  End BigStep.
-
-  Definition kstate := (list (cmd * stack) * heap)%type.
-
-  Module PLang.
-    Definition pstate := (stack * pheap)%type.
-  
-    Definition access_ok (c : cmd) (s : stack) (h : pheap) :=
-      match accesses c s with
-        | None => True
-        | Some v => exists x, this h v = Some x
-      end.
-
-    Definition write_ok (c : cmd) (s : stack) (h : pheap) :=
-      match writes c s with
-        | None => True
-        | Some v => exists x, this h v = Some (full_p, x)
-      end.
-
-    Inductive red_p: cmd -> pstate -> cmd -> pstate -> Prop :=
-      redp_ster : forall (c1 c2 : cmd) (st1 st2 : state) (pst1 pst2 : pstate) (s1 s2 : stack)
-                         (ph1 ph2 phF : pheap) (h1 h2 : heap),
-        st1 = (s1, h1) -> st2 = (s2, h2) ->
-        pst1 = (s1, ph1) -> pst2 = (s2, ph2) ->
-        access_ok c1 s1 ph1 ->
-        write_ok c1 s1 ph1 ->
-        pdisj ph1 phF -> ptoheap (phplus ph1 phF) h1 ->
-        c1 / st1 ==>s c2 / st2 ->
-        pdisj ph2 phF -> ptoheap (phplus ph2 phF) h2 ->
-        red_p c1 pst1 c2 pst2.
-    Notation "c '/' st  '==>p'  c' '/' st' " := 
-      (red_p c st c' st') (at level 40, st at level 39, c' at level 39).
-
-    Hint Resolve pdisjC.
-    Lemma Q1 (q1 q2 q : Qc) : q1 + q2 = q -> q1 = q - q2.
-    Proof. intros H; rewrite <-H; ring. Qed.
-    Hint Rewrite Q1.
-
-    Lemma Q2 (q1 q2 q : Qc) : q1 + q2 = q -> q2 = q - q1.
-    Proof. intros H; rewrite <-H; ring. Qed.
-    Hint Rewrite Q2.
-
-    Lemma phplus_cancel_toheap (ph1 ph2 phF : pheap) (h : heap):
-      pdisj ph1 phF -> pdisj ph2 phF ->
-      ptoheap (phplus ph1 phF) h -> ptoheap (phplus ph2 phF) h -> ph1 = ph2.
-    Proof.
-      intros dis1 id2 to1 to2.
-      pose proof (ptoD to1 to2).
-      eapply padd_cancel2; eauto.
-    Qed.
-
-    Lemma padd_upd_cancel (ph1 ph2 phF : pheap) (h : heap) (x v v': Z) :
-      pdisj ph1 phF -> pdisj ph2 phF -> ptoheap (phplus ph1 phF) h ->
-      this ph1 x = Some (full_p, v') -> ptoheap (phplus ph2 phF) (upd h x (Some v)) -> 
-      this ph2 = ph_upd ph1 x v.
-    Proof.
-      intros pd1 pd2 toh1 have1 toh2; extensionality y; unfold ph_upd.
-      destruct ph1 as [ph1 h1], ph2 as [ph2 h2], phF as [phF hF]; simpl in *.
-      destruct (Z.eq_dec x y).
-      - rewrite <-e; clear e y.
-        unfold is_pheap, pdisj, ptoheap, upd, phplus in *;
-          repeat (match goal with [H : forall _ : Z, _ |- _] => specialize (H x) end).
-        destruct (Z.eq_dec x x); try tauto.
-        rewrite have1 in *.
-        destruct (phF x) as [[pF vF]|]; des.
-        + apply Qcle_minus_iff in pd3.
-          cutrewrite (1 + -(full_p + pF) = -pF) in pd3; [|unfold full_p; field].
-          apply Qcopp_le_compat in pd3; ring_simplify in pd3.
-          apply Qcle_not_lt in pd3; tauto.
-        + destruct (ph2 x) as [[p2 v2]|]; try congruence.
-          des; congruence.
-      - unfold is_pheap, pdisj, ptoheap, upd, phplus in *;
-        repeat (match goal with [H : forall _ : Z, _ |- _] => specialize (H y) end).
-        destruct (Z.eq_dec y x); [symmetry in e; tauto |].
-        destruct (ph1 y) as [[? ?]|], (phF y) as [[? ?]|], (ph2 y) as [[? ?]|]; des; 
-        try congruence.
-        apply Q1 in toh1; apply Q1 in toh2.
-        destruct (h y) as [? | ]; inversion toh0; inversion toh3; congruence.
-        rewrite toh2 in toh1.
-        assert (q + full_p - full_p = full_p - full_p) by (rewrite toh1; ring).
-        ring_simplify in H; rewrite H in h1; inversion h1.
-        rewrite toh1 in toh2.
-        assert (q0 + full_p - full_p = full_p - full_p) by (rewrite toh2; ring).
-        ring_simplify in H; rewrite H in h2; inversion h2.
-    Qed.
-
-    Lemma red_p_det (c c1 c2 : cmd) (st st1 st2 : pstate) :
-      c / st ==>p c1 / st1 ->
-      c / st ==>p c2 / st2 ->
-      c1 = c2 /\ st1 = st2.
-    Proof.
-      intros red1 red2.
-      destruct red1 as
-          [c1 c1' st1 st1' pst1 pst1' s1 s1' ph1 ph1' phF1 h1 h1' eq1 eq1' 
-              peq1 peq1' aok1 wok1 dis1 to1 red1 dis1' to1'].
-      destruct red2 as
-          [c2 c2' st2 st2' pst2 pst2' s2 s2' ph2 ph2' phF2 h2 h2' eq2 eq2' 
-              peq2 peq2' aok2 wok2 dis2 to2 red2 dis2' to2'].
-      induction [c2' red2]red1; intros c2' red2; 
-      try (inversion red2; subst; 
-           repeat (match goal with [H : (_, _) = (_, _) |- _ ] => inversion H; subst; clear H end);
-           simpl in *; try congruence;
-           assert (ph1' = ph2) by (eapply phplus_cancel_toheap; eauto);
-           assert (ph2' = ph2) by (eapply phplus_cancel_toheap; eauto);
-           split; congruence).
-      - inversion red2; subst.
-        + repeat (match goal with [H : (_, _) = (_, _) |- _ ] => inversion H; subst; clear H end).
-          assert (ph1' = ph2) by (eapply phplus_cancel_toheap; eauto).
-          assert (ph2' = ph2) by (eapply phplus_cancel_toheap; eauto).
-          split; congruence.
-        + inversion R.
-      - inversion red2; subst. 
-        + inversion red1.
-        + unfold access_ok, write_ok in *; simpl in *. 
-          pose proof (IHred1 eq_refl eq_refl aok1 wok1 aok2 wok2 c1'0 R) as H; 
-            destruct H as [He1 He2].
-          split; [subst; eauto | eauto].
-      - inversion red2; subst;
-        repeat (match goal with [H : (_, _) = (_, _) |- _ ] => inversion H; subst; clear H end).
-        unfold access_ok in *; simpl in *.
-        remember (edenot e s0) as vad.
+      + repeat (match goal with [H : (_, _) = (_, _) |- _ ] => inversion H; subst; clear H end).
         assert (ph1' = ph2) by (eapply phplus_cancel_toheap; eauto).
         assert (ph2' = ph2) by (eapply phplus_cancel_toheap; eauto).
-        cutrewrite (v = v0); [split; congruence |].
-        assert (Some v0 = Some v) as Heq; [ rewrite <- RD0, <-RD | 
-                                            rewrite <-RD0, <-RD in Heq; congruence].
-        clear Heqvad; subst.
-        destruct aok1 as [[q va] Hv].
-        unfold pdisj, ptoheap in *.
-        repeat (match goal with [H : forall _ : Z, _ |- _] => specialize (H vad) end).
-        unfold phplus in *.
-        rewrite Hv in *.
-        destruct (this phF1 vad) as [[? ?] | ], (this phF2 vad) as [[? ?] | ]; des; try congruence.
-      - inversion red2; subst.
-        split; eauto.
-        assert (s1' = s2') by congruence; subst.
-        assert (ph1' = ph2'); [| subst; eauto].
-        inversion EQ3; inversion EQ0; inversion peq2; inversion EQ2; inversion EQ1. 
-        subst. rewrite H8 in *.
-        unfold write_ok in *; simpl in *.
-        destruct wok1 as [v1' H1], wok2 as [v2' H2].
-        remember (edenot e1 s) as addr. clear Heqaddr.
-        remember (edenot e2 s) as v. clear Heqv.
-        assert (this ph1' = ph_upd ph2 addr v) by eapply (padd_upd_cancel dis1 dis1' to1 H1 to1').
-        assert (this ph2' = ph_upd ph2 addr v) by eapply (padd_upd_cancel dis2 dis2' to2 H2 to2').
-        destruct ph1' as [ph1' h1], ph2' as [ph2' h2]; simpl in *; subst.
-        assert (h1 = h2) by apply proof_irrelevance; congruence.
-    Qed.
+        split; congruence.
+      + inversion R.
+    - inversion red2; subst. 
+      + inversion red1.
+      + unfold access_ok, write_ok in *; simpl in *. 
+        pose proof (IHred1 eq_refl eq_refl aok1 wok1 aok2 wok2 c1'0 R) as H; 
+          destruct H as [He1 He2].
+        split; [subst; eauto | eauto].
+    - inversion red2; subst;
+      repeat (match goal with [H : (_, _) = (_, _) |- _ ] => inversion H; subst; clear H end).
+      unfold access_ok in *; simpl in *.
+      remember (edenot e s0) as vad.
+      assert (ph1' = ph2) by (eapply phplus_cancel_toheap; eauto).
+      assert (ph2' = ph2) by (eapply phplus_cancel_toheap; eauto).
+      cutrewrite (v = v0); [split; congruence |].
+      assert (Some v0 = Some v) as Heq; [ rewrite <- RD0, <-RD | 
+                                          rewrite <-RD0, <-RD in Heq; congruence].
+      clear Heqvad; subst.
+      destruct aok1 as [[q va] Hv].
+      unfold pdisj, ptoheap in *.
+      repeat (match goal with [H : forall _ : Z, _ |- _] => specialize (H vad) end).
+      unfold phplus in *.
+      rewrite Hv in *.
+      destruct (this phF1 vad) as [[? ?] | ], (this phF2 vad) as [[? ?] | ]; des; try congruence.
+    - inversion red2; subst.
+      split; eauto.
+      assert (s1' = s2') by congruence; subst.
+      assert (ph1' = ph2'); [| subst; eauto].
+      inversion EQ3; inversion EQ0; inversion peq2; inversion EQ2; inversion EQ1. 
+      subst. rewrite H8 in *.
+      unfold write_ok in *; simpl in *.
+      destruct wok1 as [v1' H1], wok2 as [v2' H2].
+      remember (edenot e1 s) as addr. clear Heqaddr.
+      remember (edenot e2 s) as v. clear Heqv.
+      assert (this ph1' = ph_upd ph2 addr v) by eapply (padd_upd_cancel dis1 dis1' to1 H1 to1').
+      assert (this ph2' = ph_upd ph2 addr v) by eapply (padd_upd_cancel dis2 dis2' to2 H2 to2').
+      destruct ph1' as [ph1' h1], ph2' as [ph2' h2]; simpl in *; subst.
+      assert (h1 = h2) by apply proof_irrelevance; congruence.
+  Qed.
+End PLang.
 
-    Section Typing.
-      Inductive type := Hi | Lo.
-      Definition join (t1 t2 : type) :=
-        match (t1, t2) with
-          | (Hi, _) | (_, Hi) => Hi
-          | (Lo, Lo) => Lo
-        end.
-      
-      Definition le_type (t1 t2 : type) : bool :=
-        match (t1, t2) with
-          | (Lo, _) | (_, Hi) => true
-          | (Hi, Lo) => false
-        end.
+Module BigStep.
+  Import PLang.
+  Reserved Notation " c '/' s '||' c' '/' s'" (at level 40, s at level 39, c' at level 39).
+  Inductive eval : cmd -> pstate -> option (nat * cmd) -> pstate -> Prop :=
+  | eval_Skip : forall (st : pstate), SKIP / st || None / st
+  | eval_Seq1 : forall (c1 c2 c1': cmd) (st st' : pstate) (j : nat),
+                  c1 / st || (Some (j, c1')) / st' ->
+                  (c1 ;; c2) / st || Some (j, c1' ;; c2) / st'
+  | eval_Seq2 : forall (c1 c2 : cmd) (c2' : option (nat * cmd)) (st st' st'' : pstate), 
+                  c1 / st || None / st' -> c2 / st' || c2' / st'' -> (c1 ;; c2) / st || c2' / st''
+  | eval_If1 : forall (b : bexp) (c1 c2 : cmd) (c1' : option (nat * cmd)) (st st' : pstate),
+                 bdenot b (fst st) = true -> c1 / st || c1' / st' ->
+                 (Cif b c1 c2) / st || c1' / st'
+  | eval_If2 : forall (b : bexp) (c1 c2 : cmd) (c2' : option (nat * cmd)) (st st' : pstate),
+                 bdenot b (fst st) = false -> c2 / st || c2' / st' ->
+                 (Cif b c1 c2) / st || c2' / st'
+  | eval_Loop : forall (b : bexp) (c : cmd) (c' : option (nat * cmd)) (st st' : pstate),
+                  (Cif b (c ;; (Cwhile b c)) Cskip) / st || c'/ st' ->
+                  (Cwhile b c) / st || c' / st'
+  | eval_Assign : forall (x : var) (e : exp) (st st' : pstate) s h,
+                    (st = (s, h)) -> (st' = (upd s x (edenot e s), h)) ->
+                    (x ::= e) / st || None / st'
+  | eval_Read : forall (x : var) (e : exp) (v : Z) (st st' : pstate) (s : stack) (h : pheap) (q : Qc),
+                  (st = (s, h)) -> (this h (edenot e s) = Some (q, v)) ->
+                  (st' = (upd s x v, h)) ->
+                  (x ::= [e]) / st || None / st'
+  | eval_Write : forall (e1 e2 : exp) (ss ss' : pstate) (s : stack) (h : pheap) (v : Z),
+                   (ss = (s, h)) ->
+                   this h (edenot e1 s) = Some (1, v) ->
+                   (ss' = (s, ph_upd2 h (edenot e1 s) (edenot e2 s))) ->
+                   (Cwrite e1 e2) / ss || None / ss'
+  | eval_Barrier : forall ss j,
+                     (Cbarrier j) / ss || Some (j, Cskip) / ss
+                                  where " c '/' s '||' c' '/' s'" := (eval c s c' s').
+  
+  Lemma red1_eval (c1 c2 : cmd) (st1 st2 : pstate) (st : pstate) : 
+    c1 / st1 ==>p c2 / st2 -> c2 / st2 || None / st -> c1 / st1 || None / st.
+  Proof.
+    move=> H IH.
+    destruct H as
+        [c c' st' st'' pst pst' s s' ph ph' phF h h' eq eq' 
+            peq peq' aok wok dis to red dis' to'].
+    induction [st IH]red; ins; subst; 
+    repeat (match goal with [H : (_, _) = (_, _) |- _ ] => inversion H; subst; clear H end); 
+    try assert (ph = ph') by (eapply phplus_cancel_toheap; eauto); subst;
+    try (constructor; tauto).
+    - econstructor; [econstructor | eauto].
+    - inversion IH; subst; unfold access_ok, write_ok in *; simpl in *. 
+      pose proof (IHred eq_refl eq_refl aok wok _ H1).
+      econstructor; eauto.
+    - apply eval_If2; eauto.
+    - eapply eval_Assign; eauto.
+      inversion IH; subst; eauto.
+    - unfold access_ok in *; simpl in *; destruct aok as [[q v'] h].
+      eapply eval_Read; eauto.
+      inversion IH; subst.
+      unfold ptoheap, phplus in to; specialize (to (edenot e s0)); rewrite h in to;
+      destruct (this phF (edenot e s0)) as [[? ?] |]; destruct to as [? H'];
+      rewrite H' in *; inversion RD; eauto.
+    - unfold write_ok in *; simpl in *; destruct wok as [v' h];
+      eapply eval_Write; eauto.
+      inversion IH; subst; eauto.
+      cutrewrite (ph' = ph_upd2 ph (edenot e1 s0) (edenot e2 s0)); eauto.
+      assert (this ph' = this (ph_upd2 ph (edenot e1 s0) (edenot e2 s0))) by 
+          (eapply padd_upd_cancel; eauto).
+      destruct ph'; simpl in H.
+      unfold ph_upd2.
+      symmetry in H; destruct H.
+      cutrewrite (is_p = ph_upd_ph ph (edenot e1 s0) (edenot e2 s0)); 
+        [ eauto | apply proof_irrelevance ].
+  Qed.
+  (*
+  Corollary red1_eval' (c1 c2 : cmd) (st1 st2 st3 : pstate) : 
+    c1 / st1 ==>s c2 / st2 -> c2 / st2 || None / st3 -> c1 / st1 || None / st3.
+  Proof.
+    move=> H H'.
+    remember (c1, st1) as s1.
+    assert (c1 = fst s1) as h by (rewrite Heqs1; tauto); rewrite h in *; clear h.
+    assert (st1 = snd s1) as h by (rewrite Heqs1; tauto); rewrite h in *; clear h.
+    remember (c2, st2) as s2.
+    assert (c2 = fst s2) as h by (rewrite Heqs2; tauto); rewrite h in *; clear h.
+    assert (st2 = snd s2) as h by (rewrite Heqs2; tauto); rewrite h in *; clear h.
+    eapply red1_eval; eauto.
+  Qed.
+   *)
 
-      Definition env := var -> type.
-      Inductive typing_exp : env -> exp -> type -> Prop := 
-      | ty_var : forall (g : env) (v : var) (ty : type), g v = ty -> typing_exp g (Evar v) ty
-      | ty_num : forall (g : env) (n : Z) (ty : type), typing_exp g (Enum n) ty
-      | ty_plus : forall (g : env) (e1 e2 : exp) (ty1 ty2 : type), 
-                    typing_exp g e1 ty1 -> typing_exp g e2 ty2 ->
-                    typing_exp g (Eplus e1 e2) (join ty1 ty2).
+  Lemma eval__mred1 (c : cmd) (st st' : pstate) : 
+    c / st ==>p* Cskip / st' -> c / st || None / st'.
+    intros H; unfold multi_red_p in H.
+    remember (c, st) as s.
+    remember (SKIP, st') as s'.
+    assert (c = fst s) as h by (rewrite Heqs; tauto); rewrite h; clear h.
+    assert (st = snd s) as h by (rewrite Heqs; tauto); rewrite h; clear h.
+    assert (st' = snd s') as h by (rewrite Heqs'; tauto); rewrite h; clear h.
+    clear Heqs.
+    induction [Heqs'] H.
+    - move=>->; simpl; apply eval_Skip.
+    - move/IHclos_refl_trans_1n=>IH; clear IHclos_refl_trans_1n.
+      clear H0.
+      eapply red1_eval; eauto.
+  Qed.
 
-      Inductive typing_bexp : env -> bexp -> type -> Prop := 
-      | ty_eq : forall (g : env) (e1 e2 : exp) (ty1 ty2 : type), 
+  Lemma eval_mred2 (c c' c'': cmd) (st st' : pstate) (j : nat) : 
+    c / st ==>p* c' / st' -> wait c' = Some (j, c'') ->
+    c / st || Some (j, c'') / st'.
+  Proof.
+    intros hs hwait.
+    unfold multi_red_p in hs.
+    remember (c, st) as s.
+    remember (c', st') as s'.
+    assert (c = fst s) as h by (rewrite Heqs; tauto); rewrite h; clear h.
+    assert (st = snd s) as h by (rewrite Heqs; tauto); rewrite h; clear h.
+    assert (st' = snd s') as h by (rewrite Heqs'; tauto); rewrite h; clear h.
+    clear Heqs.
+    induction [Heqs'] hs.
+    - intros ->.
+      induction [c'' j hwait]c'; move=> c'' j' hwait; inversion hwait.
+      + destruct (wait c'1); eauto.
+        * destruct p as (j'', c'); simpl in *.
+          apply eval_Seq1.
+          now apply IHc'1.
+        * inversion H0.
+      + apply eval_Barrier.
+    - move=>->; simpl in *.
+      assert ((c', st') = (c', st')) as IH by eauto; apply IHhs in IH; clear IHhs; simpl in *.
+      clear hs hwait c' c st.
+      unfold red_p_tup in H.
+      destruct H as [c c' stp' stp'' pst pst' s s' ph ph' phF h h' eq eq' 
+                     peq peq' aok wok dis to red dis' to'].
+      induction [c'' IH]red; ins; subst; try inversion eq'; subst.
+      + eapply eval_Seq2; [apply eval_Skip | apply phplus_cancel_toheap].
+      + inversion IH; subst.
+        * apply eval_Seq1. 
+          apply IHred; eauto.
+        * eapply eval_Seq2; eauto.
+          eapply red1_eval'; eauto.
+      + apply eval_If2; eauto.
+      + inversion IH.
+      + inversion IH.
+      + inversion IH.
+  Qed.
+End BigStep.
+
+Definition kstate := (list (cmd * stack) * heap)%type.
+
+Module NonInter.
+  Inductive type := Hi | Lo.
+  Definition join (t1 t2 : type) :=
+      match (t1, t2) with
+        | (Hi, _) | (_, Hi) => Hi
+        | (Lo, Lo) => Lo
+      end.
+    
+    Definition le_type (t1 t2 : type) : bool :=
+      match (t1, t2) with
+        | (Lo, _) | (_, Hi) => true
+        | (Hi, Lo) => false
+      end.
+
+    Definition env := var -> type.
+    Inductive typing_exp : env -> exp -> type -> Prop := 
+    | ty_var : forall (g : env) (v : var) (ty : type), g v = ty -> typing_exp g (Evar v) ty
+    | ty_num : forall (g : env) (n : Z) (ty : type), typing_exp g (Enum n) ty
+    | ty_plus : forall (g : env) (e1 e2 : exp) (ty1 ty2 : type), 
                   typing_exp g e1 ty1 -> typing_exp g e2 ty2 ->
-                  typing_bexp g (Beq e1 e2) (join ty1 ty2)
-      | ty_and : forall (g : env) (b1 b2 : bexp) (ty1 ty2 : type), 
-                  typing_bexp g b1 ty1 -> typing_bexp g b2 ty2 ->
-                  typing_bexp g (Band b1 b2) (join ty1 ty2)
-      | ty_not : forall (g : env) (b : bexp) (ty : type), 
-                   typing_bexp g b ty -> typing_bexp g (Bnot b) ty.
+                  typing_exp g (Eplus e1 e2) (join ty1 ty2).
 
-      Inductive typing_cmd : env -> cmd -> type -> Prop :=
-      | ty_skip : forall (g : env) (pc : type), typing_cmd g Cskip pc
-      | ty_assign : forall (g : env) (v : var) (e : exp) (pc ty : type),
-                      typing_exp g e ty -> le_type (join ty pc) (g v) = true ->
-                      typing_cmd g (v ::= e) pc
-      | ty_read : forall (g : env) (v : var) (e : exp) (pc ty : type),
+    Inductive typing_bexp : env -> bexp -> type -> Prop := 
+    | ty_eq : forall (g : env) (e1 e2 : exp) (ty1 ty2 : type), 
+                typing_exp g e1 ty1 -> typing_exp g e2 ty2 ->
+                typing_bexp g (Beq e1 e2) (join ty1 ty2)
+    | ty_and : forall (g : env) (b1 b2 : bexp) (ty1 ty2 : type), 
+                 typing_bexp g b1 ty1 -> typing_bexp g b2 ty2 ->
+                 typing_bexp g (Band b1 b2) (join ty1 ty2)
+    | ty_not : forall (g : env) (b : bexp) (ty : type), 
+                 typing_bexp g b ty -> typing_bexp g (Bnot b) ty.
+
+    Inductive typing_cmd : env -> cmd -> type -> Prop :=
+    | ty_skip : forall (g : env) (pc : type), typing_cmd g Cskip pc
+    | ty_assign : forall (g : env) (v : var) (e : exp) (pc ty : type),
                     typing_exp g e ty -> le_type (join ty pc) (g v) = true ->
-                    typing_cmd g (v ::= [e]) pc
-      | ty_write : forall (g : env) (e1 e2 : exp) (pc : type),
-                     typing_cmd g ([e1] ::= e2) pc
-      | ty_seq : forall (g : env) (c1 c2 : cmd) (pc : type),
-                   typing_cmd g c1 pc -> typing_cmd g c2 pc ->
-                   typing_cmd g (c1 ;; c2) pc
-      | ty_if : forall (g : env) (b : bexp) (c1 c2 : cmd) (pc ty : type),
-                  typing_bexp g b ty ->
-                  typing_cmd g c1 (join pc ty) -> typing_cmd g c2 (join pc ty) ->
-                  typing_cmd g (Cif b c1 c2) pc
-      | ty_while : forall (g : env) (b : bexp) (c : cmd) (pc ty : type),
-                     typing_bexp g b ty ->
-                     typing_cmd g c (join pc ty) -> typing_cmd g (Cwhile b c) pc
-      | ty_barrier : forall (g : env) (j : nat), typing_cmd g (Cbarrier j) Lo.
-
-      
-
-End Language.
+                    typing_cmd g (v ::= e) pc
+    | ty_read : forall (g : env) (v : var) (e : exp) (pc ty : type),
+                  typing_exp g e ty -> le_type (join ty pc) (g v) = true ->
+                  typing_cmd g (v ::= [e]) pc
+    | ty_write : forall (g : env) (e1 e2 : exp) (pc : type),
+                   typing_cmd g ([e1] ::= e2) pc
+    | ty_seq : forall (g : env) (c1 c2 : cmd) (pc : type),
+                 typing_cmd g c1 pc -> typing_cmd g c2 pc ->
+                 typing_cmd g (c1 ;; c2) pc
+    | ty_if : forall (g : env) (b : bexp) (c1 c2 : cmd) (pc ty : type),
+                typing_bexp g b ty ->
+                typing_cmd g c1 (join pc ty) -> typing_cmd g c2 (join pc ty) ->
+                typing_cmd g (Cif b c1 c2) pc
+    | ty_while : forall (g : env) (b : bexp) (c : cmd) (pc ty : type),
+                   typing_bexp g b ty ->
+                   typing_cmd g c (join pc ty) -> typing_cmd g (Cwhile b c) pc
+    | ty_barrier : forall (g : env) (j : nat), typing_cmd g (Cbarrier j) Lo.
+End NonInter.
